iris/base_logic/bi.v
@@ -1,4 +1,5 @@
-From iris.bi Require Export derived_connectives extensions updates internal_eq plainly cmra.
+From iris.bi Require Export derived_connectives extensions
+  updates internal_eq plainly cmra.
 From iris.base_logic Require Export upred.
 From iris.prelude Require Import options.
 Import uPred_primitive.
